# 1
## a
$f(x)=x\cdot\left(1-\ln\left(x\right)\right)^2$<br>
$(\left(1-\ln\left(x\right)\right)^{2})'=-\dfrac{2\left(1-\ln\left(x\right)\right)}{x}2$<br>
$f'(x)=\left(1-\ln\left(x\right)\right)^2-2\left(1-\ln\left(x\right)\right)2$<br>
$(ln(x)+1)(ln(x)âˆ’1)=ln(x)^2-2\left(1-\ln\left(x\right)\right)=f'(x)2$<br>

## b
|   x   | 0     |      | $\frac{1}{e}$  |      | 1    |
| ---: | :---- | :--: | :--: | :---: | ----: |
| $f(x)$  | undef |  $\nearrow$   |$\frac{4}{e}$|    $\searrow$ | 1    |
| $f'(x)$ | undef |  +   |  0   |    - | -1   |
# 2
## a
environ $12.5 ua$
## b
$g(x)=ln(x)2$<br>
$d_{0,2}=\frac{1}{0.2}+ln(0.2)2$<br>
